More proofs in src/Data/Map.v

src/Data/Map.v
@@ -1,13 +1,25 @@
 Require Export
+  Coq.Arith.Arith
   Coq.Lists.List
   Coq.Bool.Bool
   Coq.Unicode.Utf8
+  Coq.micromega.Lia
   Coq.Classes.SetoidClass
   Coq.Classes.Morphisms
   Pact.Data.Eq
   Pact.Data.Ord.
 
+Require Export Equations.Prop.DepElim.
+From Equations Require Export Equations.
+
+Set Implicit Arguments.
+Unset Strict Implicit.
+Unset Printing Implicit Defensive.
+
+Set Equations With UIP.
+
 Generalizable All Variables.
+Set Primitive Projections.
 
 (** General utility library providing partial maps, built
     on a foundation isomorphic to association lists. *)
@@ -25,6 +37,12 @@ Inductive Map (k v : Type) : Type :=
 Arguments Empty {_ _}.
 Arguments Add {_ _} _ _ _.
 
+Inductive MapsTo `{Eq k} (i : k) (x : v) : Map k v -> Prop :=
+  | MapsTo_hd i' x' m :
+    i == i' = true -> x = x' → MapsTo i x (Add i' x' m)
+  | MapsTo_tl i' x' m :
+    i == i' = false → MapsTo i x m -> MapsTo i x (Add i' x' m).
+
 Fixpoint lookup `{Eq k} (i : k) (m : Map k v) : option v :=
   match m with
   | Empty => None
@@ -33,6 +51,18 @@ Fixpoint lookup `{Eq k} (i : k) (m : Map k v) : option v :=
       then Some x
       else lookup i m
   end.
+
+Lemma MapsTo_lookup `{Eq k} i x m : MapsTo i x m ↔ lookup i m = Some x.
+Proof.
+  split; intros.
+  - induction H0; simpl; subst;
+    now rewrite H0.
+  - induction m; simpl in *; [|discriminate].
+    destruct (i == k0) eqn:Heqe.
+    + inversion H0; subst.
+      now constructor.
+    + apply MapsTo_tl; auto.
+Qed.
 
 #[export]
 Program Instance Map_Typeoid `{Eq k} : Setoid (Map k v) := {|
@@ -54,20 +84,20 @@ Program Instance member_respects `{Eq k} :
   Proper (eq ==> equiv ==> eq) member.
 Next Obligation.
   repeat intro; subst.
-  specialize (H1 y).
+  specialize (H0 x).
   generalize dependent y.
   induction x0; simpl; intros.
-  - destruct (y == k0) eqn:Heqe; simpl.
+  - destruct (x == k0) eqn:Heqe; simpl.
     + apply eqb_eq in Heqe; subst.
-      clear -H1.
-      induction y0; simpl in *; auto.
+      clear -H0.
+      induction y; simpl in *; auto.
       * destruct (k0 == k1) eqn:Heqe; simpl; auto.
       * congruence.
     + now apply IHx0.
-  - induction y0; simpl in *; auto.
-    destruct (y == k0) eqn:Heqe; simpl.
+  - induction y; simpl in *; auto.
+    destruct (x == k0) eqn:Heqe; simpl.
     + congruence.
-    + now apply IHy0.
+    + now apply IHy.
 Qed.
 
 Fixpoint toList (m : Map k v) : list (k * v) :=
@@ -112,11 +142,83 @@ Next Obligation.
     discriminate.
 Qed.
 
+Fixpoint delete `{Eq k} (i : k) (m : Map k v) : Map k v :=
+  match m with
+  | Empty => m
+  | Add i' x m =>
+      if i == i'
+      then delete i m
+      else Add i' x (delete i m)
+  end.
+
+Lemma delete_idem `{Eq k} i m :
+  delete i (delete i m) = delete i m.
+Proof.
+  induction m; simpl; auto.
+  destruct (i == k0) eqn:Heqe; auto; simpl.
+  rewrite Heqe.
+  now rewrite IHm.
+Qed.
+
+Lemma delete_comm `{Eq k} i j m :
+  delete i (delete j m) = delete j (delete i m).
+Proof.
+  generalize dependent j.
+  generalize dependent i.
+  induction m; simpl; intros; auto.
+  destruct (i == k0) eqn:Heqe1; auto; simpl.
+  - destruct (j == k0) eqn:Heqe2; auto; simpl.
+    now rewrite Heqe1.
+  - destruct (j == k0) eqn:Heqe2; auto; simpl.
+    rewrite Heqe1.
+    now rewrite IHm.
+Qed.
+
 Fixpoint size (m : Map k v) : nat :=
   match m with
   | Add _ _ m => 1 + size m
   | Empty => 0
   end.
+
+Lemma size_delete `{Eq k} i m : (size (delete i m) <= size m)%nat.
+Proof.
+  induction m; simpl; auto.
+  destruct (i == k0) eqn:Heqe;
+  auto; simpl; lia.
+Qed.
+
+Equations compress `{Eq k} (m : Map k v) : Map k v by wf (size m) :=
+  compress Empty := Empty;
+  compress (Add i' x m) := Add i' x (compress (delete i' m)).
+Next Obligation.
+  specialize (compress H m).
+  pose proof (size_delete i' m); lia.
+Qed.
+
+Lemma compress_delete `{Eq k} i m :
+  compress (delete i m) = delete i (compress m).
+Proof.
+  generalize dependent i.
+  funelim (compress m); simpl; intros; auto.
+  simp compress; simpl.
+  destruct (i == i') eqn:Heqe.
+  - apply eqb_eq in Heqe; subst.
+    rewrite <- H0.
+    now rewrite delete_idem.
+  - simp compress; simpl.
+    f_equal.
+    rewrite <- H0.
+    now rewrite delete_comm.
+Qed.
+
+Lemma size_compress `{Eq k} m : (size (compress m) <= size m)%nat.
+Proof.
+  induction m; auto.
+  simp compress; simpl.
+  apply le_n_S.
+  rewrite compress_delete.
+  now rewrite size_delete.
+Qed.
 
 Fixpoint findWithDefault `{Eq k} (d : v) (i : k) (m : Map k v) : v :=
   match m with
@@ -134,11 +236,68 @@ Definition singleton (i : k) (x : v) : Map k v := Add i x empty.
 Fixpoint insert `{Eq k} (i : k) (x : v) (m : Map k v) : Map k v :=
   match m with
   | Empty => singleton i x
-  | Add i' _ m =>
+  | Add i' x' m =>
       if i == i'
       then Add i x m
-      else insert i x m
+      else Add i' x' (insert i x m)
   end.
+
+Lemma lookup_insert `{Eq k} i j x m :
+  lookup i (insert j x m) = if i == j then Some x else lookup i m.
+Proof.
+  destruct (i == j) eqn:Heqe1.
+  - induction m; simpl; intros.
+    + destruct (j == k0) eqn:Heqe2; simpl.
+      * now rewrite Heqe1.
+      * apply eqb_eq in Heqe1; subst.
+        now rewrite Heqe2.
+    + now destruct (i == j).
+  - induction m; simpl; intros.
+    + destruct (j == k0) eqn:Heqe2; simpl.
+      * rewrite Heqe1.
+        apply eqb_eq in Heqe2; subst.
+        now rewrite Heqe1.
+      * now rewrite IHm.
+    + now destruct (i == j).
+Qed.
+
+Lemma lookup_delete `{Eq k} i j m :
+  lookup i (delete j m) = if i == j then None else lookup i m.
+Proof.
+  induction m; simpl.
+  - destruct (i == j) eqn:Heqe1.
+    + destruct (j == k0) eqn:Heqe2; auto.
+      simpl.
+      apply eqb_eq in Heqe1; subst.
+      now rewrite Heqe2.
+    + destruct (j == k0) eqn:Heqe2; simpl; auto.
+      * apply eqb_eq in Heqe2; subst.
+        now rewrite Heqe1.
+      * now destruct (i == k0).
+  - now destruct (i == j).
+Qed.
+
+Lemma compress_equiv `{Eq k} m :
+  m == compress m.
+Proof.
+  funelim (compress m); repeat intro; auto.
+  simp compress; simpl.
+  rewrite <- H0.
+  rewrite lookup_delete.
+  now destruct (k0 == i').
+Qed.
+
+Lemma insert_delete `{Eq k } i x m :
+  insert i x (delete i m) == insert i x m.
+Proof.
+  induction m; simpl; intros; auto.
+  destruct (i == k0) eqn:Heqe.
+  - rewrite IHm; clear IHm.
+    now rewrite lookup_insert.
+  - simpl.
+    rewrite Heqe; simpl.
+    now rewrite IHm.
+Qed.
 
 Fixpoint insertWith `{Eq k} (f : v → v → v) (i : k) (x : v) (m : Map k v) : Map k v :=
   match m with
@@ -166,15 +325,6 @@ Fixpoint insertLookupWithKey `{Eq k} (f : k → v → v → v) (i : k) (x : v) (
       if i == i'
       then (Some x', Add i (f i x x') m)
       else insertLookupWithKey f i x m
-  end.
-
-Fixpoint delete `{Eq k} (i : k) (m : Map k v) : Map k v :=
-  match m with
-  | Empty => m
-  | Add i' x m =>
-      if i == i'
-      then delete i m
-      else Add i' x (delete i m)
   end.
 
 Fixpoint adjust `{Eq k} (f : v → v) (i : k) (m : Map k v) : Map k v :=
